Composition/Network.v
@@ -16,10 +16,8 @@ Module CompNetwork (A : NetAddr) (M1 M2 : MessageType) (BTh : ByzThreshold A)
   (BSett : ByzSetting A)
   (* TODO is using the Adv of each sub-protocol really good? *)
   (Adv1 : Adversary A M1 BTh BSett Pk1 Pt1 Ns1) (Adv2 : Adversary A M2 BTh BSett Pk2 Pt2 Ns2)
-  (* TODO this is bad! *)
-  (PSOp1 : PacketSoupOperations Pk1) (PSOp2 : PacketSoupOperations Pk2)
-  (N1 : Network.Network A M1 BTh BSett Pk1 PSOp1 Pt1 Ns1 Adv1)
-  (N2 : Network.Network A M2 BTh BSett Pk2 PSOp2 Pt2 Ns2 Adv2).
+  (N1 : Network.Network A M1 BTh BSett Pk1 Pt1 Ns1 Adv1)
+  (N2 : Network.Network A M2 BTh BSett Pk2 Pt2 Ns2 Adv2).
 
 Import BTh SCPT.
 
@@ -31,17 +29,15 @@ Module Export CNs := CompNetState A M1 M2 BTh CM Pk1 Pk2 CPk Pt1 Pt2 SCPT Ns1 Ns
 
 Module Export CAdv <: Adversary A CM BTh BSett CPk CPt CNs.
 
-Definition byz_constraints m w :=
+Definition byzConstraints m w :=
   match m with
-  | inl m1 => Adv1.byz_constraints m1 (world_proj1 w)
-  | inr m2 => Adv2.byz_constraints m2 (world_proj2 w)
+  | inl m1 => Adv1.byzConstraints m1 (world_proj1 w)
+  | inr m2 => Adv2.byzConstraints m2 (world_proj2 w)
   end.
 
 End CAdv.
 
-Module Export CPSOp : (* hide implementation *) PacketSoupOperations CPk := PacketSoupOperationsImpl CPk.
-
-Include NetworkImpl A CM BTh BSett CPk CPSOp CPt CNs CAdv.
+Include NetworkImpl A CM BTh BSett CPk CPt CNs CAdv.
 
 Definition ssd_proj1 (q : system_step_descriptor) : N1.system_step_descriptor :=
   match q with
@@ -60,7 +56,7 @@ Definition ssd_proj1 (q : system_step_descriptor) : N1.system_step_descriptor :=
   end.
 
 (* depending on the previous protocol *)
-Definition ssd_proj2 (q : system_step_descriptor) (w w' : Ns1.World) : N2.system_step_descriptor :=
+Definition ssd_proj2 (q : system_step_descriptor) (w w' : Ns1.SystemState) : N2.system_step_descriptor :=
   match q with
   | Idle => N2.Idle
   | Deliver p =>
@@ -92,14 +88,14 @@ Local Hint Rewrite -> N1.PC.In_consume N2.PC.In_consume In_consume option_map_li
 (* the definitions should be sound *)
 
 Fact ssd_proj1_sound q w :
-  let: ww := N1.next_world (ssd_proj1 q) (world_proj1 w) in
+  let: ww := N1.next_sysstate (ssd_proj1 q) (world_proj1 w) in
   forall w' (Hstep : system_step q w w'),
     N1.system_step (ssd_proj1 q) (world_proj1 w) ww /\
-    Ns1.World_rel ww (world_proj1 w').
+    Ns1.SystemState_rel ww (world_proj1 w').
 Proof.
   intros w' Hstep.
   inversion_step' Hstep; clear Hstep; simpl.
-  all: unfold world_proj1; simpl_world.
+  all: unfold world_proj1; simpl_sysstate.
   - split; [ constructor | ]; reflexivity.
   - destruct msg as [ mRB | mAC ]; simpl.
     + unfold stmap_proj1.
@@ -162,34 +158,34 @@ Proof.
       setoid_rewrite In_sendout1. firstorder. subst. discriminate.
 Qed.
 
-Corollary reachable_proj1 w (Hr : reachable w) (Hbyz_rel : forall m, Ns1.World_rel_cong (Adv1.byz_constraints m)) :
-  exists ww, Ns1.World_rel ww (world_proj1 w) /\ N1.reachable ww.
+Corollary reachable_proj1 w (Hr : reachable w) (Hbyz_rel : forall m, Ns1.SystemState_rel_cong (Adv1.byzConstraints m)) :
+  exists ww, Ns1.SystemState_rel ww (world_proj1 w) /\ N1.reachable ww.
 Proof.
   induction Hr as [ | q w w' Hstep Hr (ww & Hrel & Hr') ].
-  - exists Ns1.initWorld. split; [ | now constructor ]. split; auto; try reflexivity.
+  - exists Ns1.initSystemState. split; [ | now constructor ]. split; auto; try reflexivity.
   - pose proof (ssd_proj1_sound Hstep) as (Ha & Hb).
-    symmetry in Hrel. pose proof Hrel as Hrel_. eapply N1.step_mirrors_World_rel in Hrel.
-    2: apply Ha. 2: auto. 2: now apply N1.next_world_preserves_World_rel.
+    symmetry in Hrel. pose proof Hrel as Hrel_. eapply N1.step_mirrors_SystemState_rel in Hrel.
+    2: apply Ha. 2: auto. 2: now apply N1.next_sysstate_preserves_SystemState_rel.
     eexists. split. 2: eapply N1.ReachableStep; try apply Hrel. all: auto.
-    rewrite <- Hb. now apply N1.next_world_preserves_World_rel. (* HMM ...? *)
+    rewrite <- Hb. now apply N1.next_sysstate_preserves_SystemState_rel. (* HMM ...? *)
 Qed.
 
-Corollary always_holds_proj1_apply w (Hr : reachable w) (Hbyz_rel : forall m, Ns1.World_rel_cong (Adv1.byz_constraints m))
-  (P : Ns1.World -> Prop) (HP : Ns1.World_rel_cong P) (Hinv : N1.always_holds P) : P (world_proj1 w).
+Corollary always_holds_proj1_apply w (Hr : reachable w) (Hbyz_rel : forall m, Ns1.SystemState_rel_cong (Adv1.byzConstraints m))
+  (P : Ns1.SystemState -> Prop) (HP : Ns1.SystemState_rel_cong P) (Hinv : N1.always_holds P) : P (world_proj1 w).
 Proof.
   pose proof (reachable_proj1 Hr Hbyz_rel) as (ww & Hrel & Hr'). apply Hinv in Hr'. apply HP in Hrel. tauto.
 Qed.
 
 Fact ssd_proj2_sound q w :
-  let: qq := ssd_proj2 q (world_proj1 w) (world_proj1 (next_world q w)) in
-  let: ww := N2.next_world qq (world_proj2 w) in
+  let: qq := ssd_proj2 q (world_proj1 w) (world_proj1 (next_sysstate q w)) in
+  let: ww := N2.next_sysstate qq (world_proj2 w) in
   forall w' (Hstep : system_step q w w'),
     N2.system_step qq (world_proj2 w) ww /\
-    Ns2.World_rel ww (world_proj2 w').
+    Ns2.SystemState_rel ww (world_proj2 w').
 Proof.
   intros w' Hstep.
   inversion_step' Hstep; clear Hstep; simpl.
-  all: unfold world_proj2; simpl_world.
+  all: unfold world_proj2; simpl_sysstate.
   - split; [ constructor | ]; reflexivity.
   - destruct msg as [ mRB | mAC ]; simpl.
     + unfold stmap_proj1.
@@ -296,20 +292,20 @@ Proof.
 Qed.
 
 (* TODO simply repeating the proof above *)
-Corollary reachable_proj2 w (Hr : reachable w) (Hbyz_rel : forall m, Ns2.World_rel_cong (Adv2.byz_constraints m)) :
-  exists ww, Ns2.World_rel ww (world_proj2 w) /\ N2.reachable ww.
+Corollary reachable_proj2 w (Hr : reachable w) (Hbyz_rel : forall m, Ns2.SystemState_rel_cong (Adv2.byzConstraints m)) :
+  exists ww, Ns2.SystemState_rel ww (world_proj2 w) /\ N2.reachable ww.
 Proof.
   induction Hr as [ | q w w' Hstep Hr (ww & Hrel & Hr') ].
-  - exists Ns2.initWorld. split; [ | now constructor ]. split; auto; try reflexivity.
+  - exists Ns2.initSystemState. split; [ | now constructor ]. split; auto; try reflexivity.
   - pose proof (ssd_proj2_sound Hstep) as (Ha & Hb).
-    symmetry in Hrel. pose proof Hrel as Hrel_. eapply N2.step_mirrors_World_rel in Hrel.
-    2: apply Ha. 2: auto. 2: now apply N2.next_world_preserves_World_rel.
+    symmetry in Hrel. pose proof Hrel as Hrel_. eapply N2.step_mirrors_SystemState_rel in Hrel.
+    2: apply Ha. 2: auto. 2: now apply N2.next_sysstate_preserves_SystemState_rel.
     eexists. split. 2: eapply N2.ReachableStep; try apply Hrel. all: auto.
-    rewrite <- Hb. now apply N2.next_world_preserves_World_rel.
+    rewrite <- Hb. now apply N2.next_sysstate_preserves_SystemState_rel.
 Qed.
 
-Corollary always_holds_proj2_apply w (Hr : reachable w) (Hbyz_rel : forall m, Ns2.World_rel_cong (Adv2.byz_constraints m))
-  (P : Ns2.World -> Prop) (HP : Ns2.World_rel_cong P) (Hinv : N2.always_holds P) : P (world_proj2 w).
+Corollary always_holds_proj2_apply w (Hr : reachable w) (Hbyz_rel : forall m, Ns2.SystemState_rel_cong (Adv2.byzConstraints m))
+  (P : Ns2.SystemState -> Prop) (HP : Ns2.SystemState_rel_cong P) (Hinv : N2.always_holds P) : P (world_proj2 w).
 Proof.
   pose proof (reachable_proj2 Hr Hbyz_rel) as (ww & Hrel & Hr'). apply Hinv in Hr'. apply HP in Hrel. tauto.
 Qed.
