Protocols/PB/Liveness.v
@@ -20,27 +20,27 @@ Import PBP.TSS.
 
 Set Implicit Arguments. (* anyway *)
 
-Definition all_echoes src r w : Prop := forall n, is_byz n = false -> (w @ n).(echoed) (src, r) = Some (value_bft src r).
+Definition all_echoes src r w : Prop := forall n, isByz n = false -> (w @ n).(echoed) (src, r) = Some (value_bft src r).
 
 Module Termination.
 
 Section Proof_of_Termination.
 
   Variables (src : Address) (r : Round).
-  Hypothesis (Hnonbyz_src : is_byz src = false) (Hex : ex_validate r (value_bft src r).1 (value_bft src r).2).
+  Hypothesis (Hnonbyz_src : isByz src = false) (Hex : ex_validate r (value_bft src r).1 (value_bft src r).2).
 
   (* TODO template based on Proof_of_Validity, Round1 *)
   Section Round1.
 
-  Variable (w : World).
+  Variable (w : SystemState).
   Hypotheses (H_w_reachable : reachable w) (Hstart : (w @ src).(sent) r).
 
   Let initmsg_in n used := In (mkP src n (InitMsg r (value_bft src r).1 (value_bft src r).2) used).
 
   Definition pkts_needed_in_round_1 pkts : Prop := Eval unfold initmsg_in in
-    incl pkts (sentMsgs w) /\
+    incl pkts (packetSoup w) /\
     Forall good_packet pkts /\ (* since pkts is under-specified *)
-    (forall n, is_byz n = false ->
+    (forall n, isByz n = false ->
       exists used, initmsg_in n used pkts).
 
   Lemma round_1_pkts : exists pkts, pkts_needed_in_round_1 pkts.
@@ -48,7 +48,7 @@ Section Proof_of_Termination.
     unfold pkts_needed_in_round_1. saturate.
     exists (List.filter (fun p =>
       (Message_eqdec p.(msg) (InitMsg r (value_bft src r).1 (value_bft src r).2)) &&
-      (Address_eqdec (P0.src p) src) && (negb (is_byz p.(dst)))) (sentMsgs w)).
+      (Address_eqdec (P0.src p) src) && (negb (isByz p.(dst)))) (packetSoup w)).
     split_and?; auto using incl_filter.
     - apply Forall_forall. intros [ s d m b ] (Hin & Hcheck)%filter_In. simpl in Hcheck. 
       autorewrite with booldec in Hcheck. hnf. simpl. eqsolve.
@@ -61,9 +61,9 @@ Section Proof_of_Termination.
   Hypotheses (Hround1 : pkts_needed_in_round_1 pkts).
 
   Definition round_1_end w' := Eval unfold initmsg_in in
-    forall n, is_byz n = false -> initmsg_in n true (sentMsgs w').
+    forall n, isByz n = false -> initmsg_in n true (packetSoup w').
 
-  Fact round_1_end_suffcond w' (Hincl : incl (map markRcv pkts) (sentMsgs w')) :
+  Fact round_1_end_suffcond w' (Hincl : incl (map markRcv pkts) (packetSoup w')) :
     round_1_end w'.
   Proof.
     destruct Hround1 as (_ & _ & H2). 
@@ -71,7 +71,7 @@ Section Proof_of_Termination.
     destruct H2 as (? & H2). now apply (in_map markRcv), Hincl in H2.
   Qed.
 
-  Lemma round_2_start_suffcond w0 l0 (Htrace0 : system_trace w l0) (Ew0 : w0 = final_world w l0) 
+  Lemma round_2_start_suffcond w0 l0 (Htrace0 : system_trace w l0) (Ew0 : w0 = final_sysstate w l0) 
     (Hw0 : round_1_end w0) : all_echoes src r w0.
   Proof.
     pose proof (reachable_by_trace Htrace0 H_w_reachable) as H_w0_reachable. rewrite <- Ew0 in H_w0_reachable.
@@ -87,15 +87,15 @@ Section Proof_of_Termination.
 
   Section Round2.
 
-  Variable (w : World).
+  Variable (w : SystemState).
   Hypotheses (H_w_reachable : reachable w) (Hstart : all_echoes src r w).
 
   Let echomsg_in n used := In (mkP n src (EchoMsg r (light_sign (r, (value_bft src r).1) (lightkey_map n))) used).
 
   Definition pkts_needed_in_round_2 pkts : Prop := Eval unfold echomsg_in in
-    incl pkts (sentMsgs w) /\
+    incl pkts (packetSoup w) /\
     Forall good_packet pkts /\ (* since pkts is under-specified *)
-    (forall n, is_byz n = false ->
+    (forall n, isByz n = false ->
       exists used, echomsg_in n used pkts).
 
   Lemma round_2_pkts : exists pkts, pkts_needed_in_round_2 pkts.
@@ -103,9 +103,9 @@ Section Proof_of_Termination.
     unfold pkts_needed_in_round_2. saturate.
     exists (List.filter (fun p => 
       match p.(msg) with
-      | EchoMsg _ _ => (negb (is_byz (P0.src p))) && (negb (is_byz p.(dst)))
+      | EchoMsg _ _ => (negb (isByz (P0.src p))) && (negb (isByz p.(dst)))
       | _ => false
-      end) (sentMsgs w)).
+      end) (packetSoup w)).
     split_and?; auto using incl_filter.
     - apply Forall_forall. intros [ s d [] b ] (Hin & Hcheck)%filter_In; try discriminate. simpl in Hcheck. 
       now autorewrite with booldec in Hcheck.
@@ -118,9 +118,9 @@ Section Proof_of_Termination.
   Hypotheses (Hround2 : pkts_needed_in_round_2 pkts).
 
   Definition round_2_end w' := Eval unfold echomsg_in in
-    forall n, is_byz n = false -> echomsg_in n true (sentMsgs w').
+    forall n, isByz n = false -> echomsg_in n true (packetSoup w').
 
-  Fact round_2_end_suffcond w' (Hincl : incl (map markRcv pkts) (sentMsgs w')) :
+  Fact round_2_end_suffcond w' (Hincl : incl (map markRcv pkts) (packetSoup w')) :
     round_2_end w'.
   Proof.
     destruct Hround2 as (_ & _ & H2). 
@@ -128,7 +128,7 @@ Section Proof_of_Termination.
     destruct H2 as (? & H2). now apply (in_map markRcv), Hincl in H2.
   Qed.
 
-  Lemma src_outputs_suffcond w0 l0 (Htrace0 : system_trace w l0) (Ew0 : w0 = final_world w l0) 
+  Lemma src_outputs_suffcond w0 l0 (Htrace0 : system_trace w l0) (Ew0 : w0 = final_sysstate w l0) 
     (Hw0 : round_2_end w0) : (w0 @ src).(output) r.
   Proof.
     pose proof (reachable_by_trace Htrace0 H_w_reachable) as H_w0_reachable. rewrite <- Ew0 in H_w0_reachable.
@@ -137,7 +137,7 @@ Section Proof_of_Termination.
     hnf in Hw0. destruct (output _ _) eqn:E; auto.
     pick output_none as_ H1 by_ (pose proof (Hst src) as []). saturate_assumptions! in_ H1.
     (* prove contradiction using the message size *)
-    assert (incl (List.filter (fun n => negb (is_byz n)) valid_nodes) (map fst ((w0 @ src).(counter) r))) as Hincl.
+    assert (incl (List.filter (fun n => negb (isByz n)) valid_nodes) (map fst ((w0 @ src).(counter) r))) as Hincl.
     { hnf. intros n1 Hnonbyz_n1%is_nonbyz_synonym. specialize (Hw0 _ Hnonbyz_n1).
       pick echomsg_recv_h2l as_ H2 by_ (pose proof (Hh2l _ Hw0) as []). saturate_assumptions. destruct H2 as [ | H2 ]; auto. 
       specialize (H2 ltac:(assumption) ltac:(now apply lightkey_correct)). now apply (in_map fst) in H2. }
