Protocols/RB/Network.v
@@ -14,7 +14,7 @@ Module RBAdversary (A : NetAddr) (R : Round) (V : Value) (VBFT : ValueBFT A R V)
 
 Import A R V VBFT BTh BSett M P RBP Ns.
 
-Definition byz_constraints (m : Message) (w : World) : Prop :=
+Definition byzConstraints (m : Message) (w : SystemState) : Prop :=
   (* no constraint here, since we assume reliable communication channels *)
   True.
 
@@ -28,40 +28,11 @@ Import A R V VBFT BTh BSett.
 (* Module Export BTh <: ClassicByzThreshold A := ClassicByzThresholdImpl A. *)
 Module Export M <: MessageType := EmptyModule <+ RBMessage A R V.
 Module Export P <: SimplePacket A M := EmptyModule <+ SimplePacket A M.
-Module Export PSOp : (* hide implementation *) PacketSoupOperations P := PacketSoupOperationsImpl P.
 Module Export RBP <: Protocol A M P BTh <: RBProtocol A R V VBFT BTh M P :=
   EmptyModule <+ RBProtocol A R V VBFT BTh M P.
 Module Export Ns <: NetState A M P BTh RBP := EmptyModule <+ NetState A M P BTh RBP.
 Module Export RBAdv <: Adversary A M BTh BSett P RBP Ns := RBAdversary A R V VBFT BTh BSett M P RBP Ns.
 
-Include NetworkImpl A M BTh BSett P PSOp RBP Ns RBAdv.
-(*
-Definition lift_node_coh_ (P : State -> Prop) : PacketSoup -> State -> Prop :=
-  fun _ st => P st.
+Include NetworkImpl A M BTh BSett P RBP Ns RBAdv.
 
-Definition lift_node_inv (P : PacketSoup -> State -> Prop) : World -> Prop :=
-  fun w => forall n, is_byz n = false ->
-    P (sentMsgs w) (localState w n).
-
-Definition lift_node_coh (P : State -> Prop) : World -> Prop :=
-  Eval unfold lift_node_inv, lift_node_coh_ in lift_node_inv (lift_node_coh_ P).
-
-Definition lift_psent_inv_ (P : StateMap -> PacketSoup -> PacketSoup -> Prop)
-  : StateMap -> PacketSoup -> Prop :=
-  fun stmap psent => P stmap psent psent.
-
-Definition lift_psent_inv (P : StateMap -> PacketSoup -> PacketSoup -> Prop)
-  : World -> Prop :=
-  Eval unfold lift_psent_inv_ in fun w => lift_psent_inv_ P (localState w) (sentMsgs w).
-
-Definition id_coh w : Prop := 
-  forall n, is_byz n = false -> (localState w n).(id) = n.
-*)
 End RBNetworkType.
-
-Module RBNetwork (A : NetAddr) (R : Round) (V : Value) (VBFT : ValueBFT A R V) 
-  (BTh : ClassicByzThreshold A) (BSett : ByzSetting A) <: RBNetworkType A R V VBFT BTh BSett.
-
-Include RBNetworkType A R V VBFT BTh BSett.
-
-End RBNetwork.
