Properties/Liveness.v
@@ -6,26 +6,26 @@ From Bythos.Systems Require Export Network.
 
 Module Liveness (Export A : NetAddr) (Export M : MessageType)
   (Export BTh : ByzThreshold A) (Export BSett : ByzSetting A) 
-  (Export P : SimplePacket A M) (Export PSOp : PacketSoupOperations P)
+  (Export P : SimplePacket A M)
   (Export Pr : Protocol A M P BTh) (Export Ns : NetState A M P BTh Pr)
-  (Export Adv : Adversary A M BTh BSett P Pr Ns) (Export N : Network A M BTh BSett P PSOp Pr Ns Adv).
+  (Export Adv : Adversary A M BTh BSett P Pr Ns) (Export N : Network A M BTh BSett P Pr Ns Adv).
 
-Definition pkts_multi_to_all size w nonbyz_senders pkts (m : Address -> Message) (P : World -> Address -> Prop) : Prop :=
+Definition pkts_multi_to_all size w nonbyz_senders pkts (m : Address -> Message) (P : SystemState -> Address -> Prop) : Prop :=
   List.NoDup nonbyz_senders /\
   size <= length nonbyz_senders /\
-  incl pkts (sentMsgs w) /\
+  incl pkts (packetSoup w) /\
   Forall good_packet pkts /\ (* since pkts is under-specified *)
   (forall n1,
     In n1 nonbyz_senders -> 
-    is_byz n1 = false /\
+    isByz n1 = false /\
     P w n1 /\
-    (forall n2, is_byz n2 = false ->
+    (forall n2, isByz n2 = false ->
       exists used, In (mkP n1 n2 (m n1) used) pkts)).
 
 Definition mutual_receiving m w' :=
-  forall n1, is_byz n1 = false -> 
-    forall n2, is_byz n2 = false ->
-      In (mkP n1 n2 (m n1) true) (sentMsgs w').
+  forall n1, isByz n1 = false -> 
+    forall n2, isByz n2 = false ->
+      In (mkP n1 n2 (m n1) true) (packetSoup w').
 
 End Liveness.
 
